src/lowparse/pulse/LowParse.Pulse.Combinators.fst
@@ -399,12 +399,13 @@ let nondep_then_eq_dtuple2
 
 inline_for_extraction
 ```pulse
-fn validate_nondep_then_cont_success2
-  (#t1 #t2: Type0)
+fn validate_dtuple2_cont_success2
+  (#t1: Type0)
+  (#t2: t1 -> Type0)
   (#k1: parser_kind)
   (p1: parser k1 t1)
   (#k2: parser_kind)
-  (p2: parser k2 t2)
+  (p2: ((x: t1) -> parser k2 (t2 x)))
   (input: slice byte)
   (offset: SZ.t)
   (#pm: perm)
@@ -412,27 +413,28 @@ fn validate_nondep_then_cont_success2
   (pre: vprop)
   (t': Type0)
   (post: (t' -> vprop))
-  (off: SZ.t {validator_success p1 offset v off /\ SZ.fits (SZ.v offset + SZ.v off) })
-  (ksucc: ((off: SZ.t) -> stt t' (pts_to input #pm v ** pre ** pure (validator_success (tot_nondep_then p1 p2) offset v off)) (fun x -> post x)))
+  (key: Ghost.erased t1)
+  (off: SZ.t { validator_success p1 offset v off /\ SZ.fits (SZ.v offset + SZ.v off) /\ fst (Some?.v (parse p1 (Seq.slice v (SZ.v offset) (Seq.length v)))) == Ghost.reveal key })
+  (ksucc: ((off: SZ.t) -> stt t' (pts_to input #pm v ** pre ** pure (validator_success (tot_parse_dtuple2 p1 p2) offset v off)) (fun x -> post x)))
   (off': SZ.t)
-  requires pts_to input #pm v ** pre ** pure (validator_success p2 (offset `SZ.add` off) v off')
+  requires pts_to input #pm v ** pre ** pure (validator_success (p2 key) (offset `SZ.add` off) v off')
   returns x: t'
   ensures post x
 {
   pts_to_len input; // for SZ.fits (off + off')
-  nondep_then_eq #k1 #t1 p1 #k2 #t2 p2 (Seq.slice v (SZ.v offset) (Seq.length v));
   ksucc (off `SZ.add` off')
 }
 ```
 
 inline_for_extraction
 ```pulse
-fn validate_nondep_then_cont_failure2
-  (#t1 #t2: Type0)
+fn validate_dtuple2_cont_failure2
+  (#t1: Type0)
+  (#t2: t1 -> Type0)
   (#k1: parser_kind)
   (p1: parser k1 t1)
   (#k2: parser_kind)
-  (p2: parser k2 t2)
+  (p2: ((x: t1) -> parser k2 (t2 x)))
   (input: slice byte)
   (offset: SZ.t)
   (#pm: perm)
@@ -440,56 +442,60 @@ fn validate_nondep_then_cont_failure2
   (pre: vprop)
   (t': Type0)
   (post: (t' -> vprop))
-  (off: SZ.t {validator_success p1 offset v off /\ SZ.fits (SZ.v offset + SZ.v off) })
-  (kfail: (unit -> stt t' (pts_to input #pm v ** pre ** pure (validator_failure (tot_nondep_then p1 p2) offset v)) (fun x -> post x)))
+  (key: Ghost.erased t1)
+  (off: SZ.t { validator_success p1 offset v off /\ SZ.fits (SZ.v offset + SZ.v off) /\ fst (Some?.v (parse p1 (Seq.slice v (SZ.v offset) (Seq.length v)))) == Ghost.reveal key })
+  (kfail: (unit -> stt t' (pts_to input #pm v ** pre ** pure (validator_failure (tot_parse_dtuple2 p1 p2) offset v)) (fun x -> post x)))
   (_: unit)
-  requires pts_to input #pm v ** pre ** pure (validator_failure p2 (offset `SZ.add` off) v)
+  requires pts_to input #pm v ** pre ** pure (validator_failure (p2 key) (offset `SZ.add` off) v)
   returns x: t'
   ensures post x
 {
-  nondep_then_eq #k1 #t1 p1 #k2 #t2 p2 (Seq.slice v (SZ.v offset) (Seq.length v));
   kfail ()
 }
 ```
 
 inline_for_extraction
 ```pulse
-fn validate_nondep_then_cont_success1
-  (#t1 #t2: Type0)
+fn validate_dtuple2_cont_success1
+  (#t1: Type0)
+  (#t2: t1 -> Type0)
   (#k1: parser_kind)
   (p1: parser k1 t1)
   (#k2: parser_kind)
-  (#p2: parser k2 t2)
-  (v2: validator p2)
+  (p2: ((x: t1) -> parser k2 (t2 x)))
   (input: slice byte)
   (offset: SZ.t)
   (#pm: perm)
   (#v: Ghost.erased bytes)
+  (v2: (off: SZ.t { validator_success p1 offset v off /\ SZ.fits (SZ.v offset + SZ.v off) }) -> (key: Ghost.erased t1 { fst (Some?.v (parse p1 (Seq.slice v (SZ.v offset) (Seq.length v)))) == Ghost.reveal key }) ->
+  validator_for (p2 key) input (SZ.add offset off) pm v)
   (pre: vprop)
   (t': Type0)
   (post: (t' -> vprop))
-  (ksucc: ((off: SZ.t) -> stt t' (pts_to input #pm v ** pre ** pure (validator_success (tot_nondep_then p1 p2) offset v off)) (fun x -> post x)))
-  (kfail: (unit -> stt t' (pts_to input #pm v ** pre ** pure (validator_failure (tot_nondep_then p1 p2) offset v)) (fun x -> post x)))
+  (ksucc: ((off: SZ.t) -> stt t' (pts_to input #pm v ** pre ** pure (validator_success (tot_parse_dtuple2 p1 p2) offset v off)) (fun x -> post x)))
+  (kfail: (unit -> stt t' (pts_to input #pm v ** pre ** pure (validator_failure (tot_parse_dtuple2 p1 p2) offset v)) (fun x -> post x)))
   (off: SZ.t)
   requires pts_to input #pm v ** pre ** pure (validator_success p1 offset v off)
   returns x: t'
   ensures post x
 {
-  pts_to_len input; // for SZ.fits (offset + off)  
-  v2 input (offset `SZ.add` off) #pm #v pre t' post
-    (validate_nondep_then_cont_success2 p1 p2 input offset #pm #v pre t' post off ksucc)
-    (validate_nondep_then_cont_failure2 p1 p2 input offset #pm #v pre t' post off kfail)
+  pts_to_len input; // for SZ.fits (offset + off)
+  let key : Ghost.erased t1 = Ghost.hide (fst (Some?.v (parse p1 (Seq.slice v (SZ.v offset) (Seq.length v)))));
+  v2 off key pre t' post
+    (validate_dtuple2_cont_success2 p1 p2 input offset #pm #v pre t' post key off ksucc)
+    (validate_dtuple2_cont_failure2 p1 p2 input offset #pm #v pre t' post key off kfail)
 }
 ```
 
 inline_for_extraction
 ```pulse
-fn validate_nondep_then_cont_failure1
-  (#t1 #t2: Type0)
+fn validate_dtuple2_cont_failure1
+  (#t1: Type0)
+  (#t2: t1 -> Type0)
   (#k1: parser_kind)
   (p1: parser k1 t1)
   (#k2: parser_kind)
-  (p2: parser k2 t2)
+  (p2: ((x: t1) -> parser k2 (t2 x)))
   (input: slice byte)
   (offset: SZ.t)
   (#pm: perm)
@@ -497,20 +503,48 @@ fn validate_nondep_then_cont_failure1
   (pre: vprop)
   (t': Type0)
   (post: (t' -> vprop))
-  (kfail: (unit -> stt t' (pts_to input #pm v ** pre ** pure (validator_failure (tot_nondep_then p1 p2) offset v)) (fun x -> post x)))
+  (kfail: (unit -> stt t' (pts_to input #pm v ** pre ** pure (validator_failure (tot_parse_dtuple2 p1 p2) offset v)) (fun x -> post x)))
   (_: unit)
   requires pts_to input #pm v ** pre ** pure (validator_failure p1 offset v)
   returns x: t'
   ensures post x
 {
-  nondep_then_eq #k1 #t1 p1 #k2 #t2 p2 (Seq.slice v (SZ.v offset) (Seq.length v));
   kfail ()
 }
 ```
 
 inline_for_extraction
 ```pulse
-fn validate_nondep_then
+fn validate_dtuple2_gen
+  (#t1: Type0)
+  (#t2: t1 -> Type0)
+  (#k1: parser_kind)
+  (#p1: parser k1 t1)
+  (v1: validator p1)
+  (#k2: parser_kind)
+  (p2: ((x: t1) -> parser k2 (t2 x)))
+  (input: slice byte)
+  (offset: SZ.t)
+  (pm: perm)
+  (v: Ghost.erased bytes)
+  (v2: (off: SZ.t { validator_success p1 offset v off /\ SZ.fits (SZ.v offset + SZ.v off) }) -> (key: Ghost.erased t1 { fst (Some?.v (parse p1 (Seq.slice v (SZ.v offset) (Seq.length v)))) == Ghost.reveal key }) ->
+  validator_for (p2 key) input (SZ.add offset off) pm v)
+: validator_for #(dtuple2 t1 t2) #(and_then_kind k1 k2) (tot_parse_dtuple2 #k1 #t1 p1 #k2 #t2 p2) input offset pm v
+= 
+  (pre: vprop)
+  (t': Type0)
+  (post: (t' -> vprop))
+  (ksucc: ((off: SZ.t) -> stt t' (pts_to input #pm v ** pre ** pure (validator_success (tot_parse_dtuple2 p1 p2) offset v off)) (fun x -> post x)))
+  (kfail: (unit -> stt t' (pts_to input #pm v ** pre ** pure (validator_failure (tot_nondep_then p1 p2) offset v)) (fun x -> post x)))
+{
+  v1 input offset #pm #v pre t' post
+    (validate_dtuple2_cont_success1 p1 p2 input offset #pm #v v2 pre t' post ksucc kfail)
+    (validate_dtuple2_cont_failure1 p1 p2 input offset #pm #v pre t' post kfail)
+}
+```
+
+inline_for_extraction
+let validate_nondep_then
   (#t1 #t2: Type0)
   (#k1: parser_kind)
   (#p1: parser k1 t1)
@@ -519,22 +553,110 @@ fn validate_nondep_then
   (#p2: parser k2 t2)
   (v2: validator p2)
 : validator #(t1 & t2) #(and_then_kind k1 k2) (tot_nondep_then #k1 #t1 p1 #k2 #t2 p2)
-= 
+= Classical.forall_intro (nondep_then_eq_dtuple2 p1 p2);
+  validate_ext
+    (validate_synth
+      (fun input offset #pm #v ->
+        validate_dtuple2_gen
+          v1
+          (fun _ -> p2)
+          input
+          offset
+          pm
+          v
+          (fun off _ -> v2 input (SZ.add offset off) #pm #v)
+      )
+      pair_of_dtuple2
+    )
+    (tot_nondep_then #k1 #t1 p1 #k2 #t2 p2)    
+
+inline_for_extraction
+```pulse
+fn validate_dtuple2_payload_cont
+  (#t1: Type0)
+  (#t2: t1 -> Type0)
+  (#k1: parser_kind)
+  (#p1: parser k1 t1)
+  (s1: serializer p1)
+  (#k2: parser_kind)
+  (p2: ((x: t1) -> parser k2 (t2 x)))
+  (v2: ((x: t1) -> validator (p2 x)))
   (input: slice byte)
   (offset: SZ.t)
-  (#pm: perm)
-  (#v: Ghost.erased bytes)
+  (pm: perm)
+  (v: Ghost.erased bytes)
+  (off: SZ.t { validator_success p1 offset v off /\ SZ.fits (SZ.v offset + SZ.v off) })
+  (key: Ghost.erased t1 { fst (Some?.v (parse p1 (Seq.slice v (SZ.v offset) (Seq.length v)))) == Ghost.reveal key })
   (pre: vprop)
   (t': Type0)
   (post: (t' -> vprop))
-  (ksucc: ((off: SZ.t) -> stt t' (pts_to input #pm v ** pre ** pure (validator_success (tot_nondep_then p1 p2) offset v off)) (fun x -> post x)))
-  (kfail: (unit -> stt t' (pts_to input #pm v ** pre ** pure (validator_failure (tot_nondep_then p1 p2) offset v)) (fun x -> post x)))
+  (ksucc: ((off': SZ.t) -> stt t' (pts_to input #pm v ** pre ** pure (validator_success (p2 key) (SZ.add offset off) v off')) (fun x -> post x)))
+  (kfail: (unit -> stt t' (pts_to input #pm v ** pre ** pure (validator_failure (p2 key) (SZ.add offset off) v)) (fun x -> post x)))
+  (input_key: slice byte)
+  (x: t1 { x == Ghost.reveal key })
+  requires (pts_to_serialized s1 input_key #pm key ** (pre ** (pts_to_serialized s1 input_key #pm key @==> pts_to input #pm v)))
+  returns res: t'
+  ensures post res
 {
-  v1 input offset #pm #v pre t' post
-    (validate_nondep_then_cont_success1 p1 v2 input offset #pm #v pre t' post ksucc kfail)
-    (validate_nondep_then_cont_failure1 p1 p2 input offset #pm #v pre t' post kfail)
+  elim_stick (pts_to_serialized s1 input_key #pm key) _;
+  v2 x input (SZ.add offset off) pre t' post ksucc kfail
 }
 ```
+
+inline_for_extraction
+```pulse
+fn validate_dtuple2_payload
+  (#t1: Type0)
+  (#t2: t1 -> Type0)
+  (#k1: parser_kind)
+  (#p1: parser k1 t1)
+  (#s1: serializer p1)
+  (r1: reader s1)
+  (#k2: parser_kind)
+  (p2: ((x: t1) -> parser k2 (t2 x)))
+  (v2: ((x: t1) -> validator (p2 x)))
+  (input: slice byte)
+  (offset: SZ.t)
+  (pm: perm)
+  (v: Ghost.erased bytes)
+  (off: SZ.t { validator_success p1 offset v off /\ SZ.fits (SZ.v offset + SZ.v off) })
+  (key: Ghost.erased t1 { fst (Some?.v (parse p1 (Seq.slice v (SZ.v offset) (Seq.length v)))) == Ghost.reveal key })
+: validator_for #(t2 key) #k2 (p2 key) input (SZ.add offset off) pm v
+=
+  (pre: vprop)
+  (t': Type0)
+  (post: (t' -> vprop))
+  (ksucc: ((off': SZ.t) -> stt t' (pts_to input #pm v ** pre ** pure (validator_success (p2 key) (SZ.add offset off) v off')) (fun x -> post x)))
+  (kfail: (unit -> stt t' (pts_to input #pm v ** pre ** pure (validator_failure (p2 key) (SZ.add offset off) v)) (fun x -> post x)))
+{
+  let input' = peek_stick_gen s1 input offset off;
+  assert (pts_to_serialized s1 input' #pm key);
+  r1 input' _ t' post (validate_dtuple2_payload_cont s1 p2 v2 input offset pm v off key pre t' post ksucc kfail input')
+}
+```
+
+inline_for_extraction
+let validate_dtuple2
+  (#t1: Type0)
+  (#t2: t1 -> Type0)
+  (#k1: parser_kind)
+  (#p1: parser k1 t1)
+  (v1: validator p1)
+  (#s1: serializer p1)
+  (r1: reader s1)
+  (#k2: parser_kind)
+  (p2: ((x: t1) -> parser k2 (t2 x)))
+  (v2: ((x: t1) -> validator (p2 x)))
+: Tot (validator (tot_parse_dtuple2 p1 p2))
+= fun input offset #pm #v ->
+    validate_dtuple2_gen
+      v1
+      p2
+      input
+      offset
+      pm
+      v
+      (validate_dtuple2_payload r1 p2 v2 input offset pm v)
 
 let split_nondep_then_post'
   (#t1 #t2: Type0)
